// Copyright (c) 2022 Robert Bosch GmbH
// All rights reserved.
//
// This source code is licensed under the CC-BY-SA-4.0 license found in the
// LICENSE file in the root directory of this source tree.

# baseURI: http://bosch-cr-aes//hsbc/bot-extension
# imports: http://www.w3.org/2003/01/geo/wgs84_pos
# imports: https://pi.pauwel.be/voc/buildingelement
# imports: https://w3id.org/bot#
# prefix: bot-ext

@prefix bot-ext: <http://bosch-cr-aes//hsbc/bot-extension#> .
@prefix owl: <http://www.w3.org/2002/07/owl#> .
@prefix rdf: <http://www.w3.org/1999/02/22-rdf-syntax-ns#> .
@prefix rdfs: <http://www.w3.org/2000/01/rdf-schema#> .
@prefix xsd: <http://www.w3.org/2001/XMLSchema#> .

<http://bosch-cr-aes//hsbc/bot-extension>
  rdf:type owl:Ontology ;
  owl:imports <http://www.w3.org/2003/01/geo/wgs84_pos> ;
  owl:imports <https://pi.pauwel.be/voc/buildingelement> ;
  owl:imports <https://w3id.org/bot#> ;
  owl:versionInfo "0.1" ;
.
bot-ext:EnergyAnalyticalSpace
  rdf:type owl:Class ;
  rdfs:comment "The EnergyAnalyticalSpace stands for a  virtual space created for heat transfer analysis" ;
  rdfs:subClassOf <https://w3id.org/bot#Space> ;
.
bot-ext:HVACSpace
  rdf:type owl:Class ;
  rdfs:comment "The HVACSpace stands for a virtual space created for Heating, Ventilation and Air-Conditioning (HVAC) related calculations" ;
  rdfs:subClassOf <https://w3id.org/bot#Space> ;
.
bot-ext:Room
  rdf:type owl:Class ;
  rdfs:comment "The Room represents a room in a building, which is designed by the architects." ;
  rdfs:subClassOf <https://w3id.org/bot#Space> ;
.
bot-ext:inverseOf
  rdf:type owl:ObjectProperty ;
  rdfs:comment "The relationship between two bot interfaces which are hosted on the two sides of the  same building element, share  the same shape but have exact opposite normals." ;
  rdfs:label "inverse of" ;
.
