// Copyright (c) 2022 Robert Bosch GmbH
// All rights reserved.
//
// This source code is licensed under the CC-BY-SA-4.0 license found in the
// LICENSE file in the root directory of this source tree.

# baseURI: http://bosch-cr-aes//hsbc/control-extension
# imports: https://w3id.org/pep/
# imports: https://w3id.org/seas/ForecastingOntology
# imports: https://w3id.org/seas/OptimizationOntology
# imports: https://www.w3.org/2019/wot/hypermedia#
# prefix: control

@prefix control: <http://bosch-cr-aes//hsbc/control-extension#> .
@prefix hctl: <https://www.w3.org/2019/wot/hypermedia#> .
@prefix owl: <http://www.w3.org/2002/07/owl#> .
@prefix rdf: <http://www.w3.org/1999/02/22-rdf-syntax-ns#> .
@prefix rdfs: <http://www.w3.org/2000/01/rdf-schema#> .
@prefix ssn: <http://www.w3.org/ns/ssn/> .
@prefix ssn-ext: <http://bosch-cr-aes//hsbc/ssn-extension#> .
@prefix xsd: <http://www.w3.org/2001/XMLSchema#> .

<http://bosch-cr-aes//hsbc/control-extension>
  rdf:type owl:Ontology ;
  owl:imports <https://w3id.org/pep/> ;
  owl:imports <https://w3id.org/seas/ForecastingOntology> ;
  owl:imports <https://w3id.org/seas/OptimizationOntology> ;
  owl:imports hctl: ;
  owl:versionInfo "Extension ontologies to the SEAS ontology. specifc for the Model Predictive Control (MPC) algorithm." ;
.
control:Ambience_Pred
  rdf:type owl:Class ;
  rdfs:comment "The class Ambience_Pred stands for the the exterior ambience forecasting algorithm." ;
  rdfs:label "Exterior ambient disturbance prediction" ;
  rdfs:subClassOf control:Forecast ;
  hctl:hasTarget "https://bosch-cr-aes/hsbc/control-extension/forecasts/ambience" ;
.
control:Comfort_Optimization
  rdf:type owl:Class ;
  rdfs:comment "A class of the MPC algorithm with an optimization objective function targetting at optimizing the room comfort." ;
  rdfs:subClassOf control:OptimalControlProblem ;
  hctl:hasTarget "https://bosch-cr-aes/hsbc/control-extension/OCP/room_comfort_optimization" ;
.
control:Energy_Conservation_Optimization
  rdf:type owl:Class ;
  rdfs:comment "A class of an MPC algorithm with an optimization objective function targetting at minimizing the HVAC energy usage for the room." ;
  rdfs:subClassOf control:OptimalControlProblem ;
  hctl:hasTarget "https://bosch-cr-aes/hsbc/control-extension/OCP/room_energy_conservation" ;
.
control:Forecast
  rdf:type owl:Class ;
  rdfs:label "A collection for the forecast services of the disturbances required in the MPC algorithms." ;
  rdfs:subClassOf <https://w3id.org/seas/Forecasting> ;
.
control:Hankel_Matrix_Dynamic
  rdf:type owl:Class ;
  rdfs:comment "The class Hankel_Matrix_Dynamic represents the System Identification algorithm that deploys Hankel Matrix method to quantify the system dynamic of the building envelope." ;
  rdfs:subClassOf control:SystemIdentification ;
  hctl:hasTarget "https://bosch-cr-aes/hsbc/control-extension/SI/hankel_dynamic" ;
.
control:ModelPredictiveController
  rdf:type owl:Class ;
  rdfs:comment "A class for the controller that executes  the specific Model Predictive Control (MPC) algorithm." ;
  rdfs:label "Model Predictive Controller" ;
  rdfs:subClassOf <https://w3id.org/pep/ProcedureExecutor> ;
  rdfs:subClassOf <https://w3id.org/seas/OptimizationExecutor> ;
.
control:Occupancy_Pred
  rdf:type owl:Class ;
  rdfs:comment "The class Occupancy_Pred  represents the occupant number forecasting algorithm (disturbance from the occupants)." ;
  rdfs:label "Number of occupants forecast" ;
  rdfs:subClassOf control:Forecast ;
  hctl:hasTarget "https://bosch-cr-aes/hsbc/control-extension/forecasts/occupants" ;
.
control:OptimalControlProblem
  rdf:type owl:Class ;
  rdfs:comment "A class of the Optimal Control Problem (OCP) involved in the Model Predictive Control (MPC) algorithm." ;
  rdfs:subClassOf <https://w3id.org/pep/Procedure> ;
  rdfs:subClassOf <https://w3id.org/seas/OptimizationProcedure> ;
.
control:RC_Dynamic
  rdf:type owl:Class ;
  rdfs:comment "The class RC_Dynamic represents the System Identification algorithm that deploys Resistance and Capacitance (RC) model to quantify the system dynamic of the building envelope." ;
  rdfs:subClassOf control:SystemIdentification ;
  hctl:hasTarget "https://bosch-cr-aes/hsbc/control-extension/SI/rc_dynamic" ;
.
control:Suppy_Air_Temperature_Pred
  rdf:type owl:Class ;
  rdfs:comment "Class Supply_Air_Temperature_Pred represents the prediction algorithm for the supply air temperature from the central AHU and before entering the reheating coil  in the room." ;
  rdfs:label "Prediction of the supply air temperature before the reheating coil." ;
  rdfs:subClassOf control:Forecast ;
  hctl:hasTarget "https://bosch-cr-aes/hsbc/control-extension/forecasts/air_temperature" ;
.
control:SystemIdentification
  rdf:type owl:Class ;
  rdfs:comment "The class SystemIdentification represent the collection of system idenfitication algorithms involved in the Model Predictive Control (MPC) algorithm." ;
  rdfs:subClassOf <https://w3id.org/pep/Procedure> ;
.
